# Hello Test Site

[filename](https://www.youtube.com/embed/hjxcc6a-LXM ':include :type=iframe width=400px height=400px')

sdf sd
sd 
fs

[Next](next.md)
[hier](weiter/hier.md)
sd
fsd
 f
 sd 
 

Inline mode: $J(\theta )= \frac{1}{2m}\left( {{\theta }^{T}}{{X}^{T}}X\theta -{{\theta}^{T}}{{X}^{T}}y-{{y}^{T}}X\theta + {{y}^{T}}y \right) $ equation.

Inline mode: $J(\theta) = - \frac{1}{m} \sum_{i=1}^m [ y^{(i)}\ \log (h_\theta (x^{(i)})) + (1 - y^{(i)})\ \log (1 - h_\theta(x^{(i)}))] + \frac{\lambda}{2m}\sum_{j=1}^n \theta_j^2$ equation 2.

Display mode:
$$
J(\theta) = - \frac{1}{m} \sum_{i=1}^m [ y^{(i)}\ \log (h_\theta (x^{(i)})) + (1 - y^{(i)})\ \log (1 - h_\theta(x^{(i)}))] + \frac{\lambda}{2m}\sum_{j=1}^n \theta_j^2
$$


Display mode with tag:
$$
J(\theta) = - \frac{1}{m} \sum_{i=1}^m [ y^{(i)}\ \log (h_\theta (x^{(i)})) + (1 - y^{(i)})\ \log (1 - h_\theta(x^{(i)}))] + \frac{\lambda}{2m}\sum_{j=1}^n \theta_j^2\tag{DIS}\label{eq:dis}
$$


here the tags $\eqref{eq:dis}$

sdg er eg
 re
 ger 
sd g
dfv ds f


